\section{Interpretation}

\subsection{Definitions}

Operationally, $\emph{Heap} \sqsubseteq \emph{Loc} \times \emph{Permission}
\times \emph{Matrix} $ (a multiset), denoted with a $\sigma$.\\
Define its \emph{interpretation} to be $\emph{Loc} \rightharpoonup
\emph{Permission} \times \emph{Matrix}$ with $\star:
\emph{Heap} \times \emph{Heap} \rightharpoonup \emph{Heap}$ as follows:
\[
    (\varsigma_1 \star \varsigma_2)(l) \equiv
    \begin{cases}
        \varsigma_1(l) & \textrm{if } l \in \dom(\varsigma_1) \wedge l \notin \dom(\varsigma_2) \\
        \varsigma_2(l) & \textrm{if } l \in \dom(\varsigma_2) \wedge l \notin \dom(\varsigma_1) \\
        (f_1 + f_2, m) & \textrm{if } (f_1, m) = \varsigma_1(l) \wedge (f_2, m) = \varsigma_2(l) \wedge f_1 + f_2 \leq 1 \\
        \textrm{undefined} & \textrm{otherwise}
    \end{cases}
\]
Commutativity and associativity of $\star$ follows from that of $+$.\\
$\varsigma_1 \star \varsigma_2$ is \emph{defined} if it is for all $l \in
\dom(\varsigma_1) \cup \dom(\varsigma_2)$.\\
\textbf{Implicitly denote} $\varsigma \equiv \den{H}{}{\sigma} \equiv
\bigstar_{(l,f,m) \in \sigma} [ l \mapsto_f m ]$.\\
\\
The $n-$fold iteration for the (functional) $StepsTo$ relation, is also a (functional) relation:
\begin{align*}
    \forall n.\ \ottkw{err} &\rightarrow^n \ottkw{err}\\
    \forall n.\ \langle \sigma , v \rangle &\rightarrow^n \langle \sigma , v \rangle\\
    \langle \sigma , e \rangle &\rightarrow^0 \langle \sigma , e \rangle\\
    \langle \sigma , e \rangle &\rightarrow^{n+1} ((\langle \sigma , e \rangle \rightarrow) \rightarrow^n)
\end{align*}
Hence, all bounded iterations end in either an $\ottkw{err}$, a heap-and-expression or a
heap-and-value.

\subsection{Interpretation}

\begin{align*}
  \V{k}{ \Unit } &= \{ (\empH, \ast) \} \\
\\
    \V{k}{ \Bool } &= \{ (\empH, true), (\empH, false) \} \\
\\
    \V{k}{ \Int } &= \{ (\empH, n) \mid 2^{-63} \leq n \leq 2^{63} -1 \} \\
\\
    \V{k}{ \Elt } &= \{ (\empH, f) \mid f \textrm{ a IEEE Float64 } \} \\
\\
    \V{k}{ f \, \Mat } &= \{ (\{ l \mapsto_{2^{-f}} \_ \} , l) \} \\
\\
    \V{k}{ \Bang t } &= \{ (\empH, \Many\, v) \mid (\empH, v) \in \V{k}{t} \} \\
\\
    \V{k}{ \forall fc.\  t } &= \{ (\varsigma, \ottkw{fun}\, fc \rightarrow \, v) \mid \forall f.\ (\varsigma, (\ottkw{fun}\, fc \rightarrow \, v)\, [ f ]) \in \V{k}{ t [ fc / f ] } \} \\
\\
    \V{k}{ t_1 \otimes t_2 } &= \{ (\varsigma_1 \star \varsigma_2, ( v_1, v_2 )) \mid (\varsigma_1, v_1) \in \V{k}{t_1} \wedge (\varsigma_2, v_2) \in \V{k}{t_2} \} \\
\\
    \V{k}{ t \multimap t' } &= \{ (\varsigma, v' ) \mid ( v' = \ottkw{fun}\, x : t \rightarrow e \vee v' = \ottkw{fix} (g, x : t, e : t') ) \, \wedge\\
                            & \qquad \qquad \forall j < k, (\varsigma_v, v) \in \V{j}{ t }.\ \varsigma \star \varsigma_v \textrm{ defined } \Rightarrow (\varsigma \star \varsigma_v, v'\, v) \in \C{j}{ t' } \} \\
\\
    \C{k}{ t } &= \{ (\varsigma_s, e) \mid \forall \, j \leq k, \sigma_r.\ \varsigma_s \star \varsigma_r \textrm{ defined } \Rightarrow \langle \sigma_s + \sigma_r, e \rangle \rightarrow^j \ottkw{err}\ \vee \exists \sigma_f, e'.\\
               & \qquad \qquad \langle \sigma_s + \sigma_r, e \rangle \rightarrow^j \langle \sigma_f + \sigma_r, e' \rangle \wedge ( e' \textrm { is a value } \Rightarrow ( \varsigma_f \star \varsigma_r, e' ) \in \V{k-j}{t} ) \} \\
\\
    \den{I}{k}{ \cdot } \theta &= \{ [] \} \\
\\
    \den{I}{k}{ \Delta, x : t } \theta &= \{ \delta[x \mapsto v_x ] \mid \delta \in \den{I}{k}{\Delta}\theta \wedge (\empH, v_x) \in \V{k}{\theta(t)} \} \\
\\
    \den{L}{k}{ \cdot } \theta &= \{ (\empH, []) \} \\
\\
    \den{L}{k}{ \Gamma, x : t } \theta &= \{ (\varsigma \star \varsigma_x, \gamma[x \mapsto v_x ]) \mid (\varsigma, \gamma) \in \den{L}{k}{\Gamma}\theta \wedge (\varsigma_x, v_x) \in \V{k}{\theta(t)} \} \\
\\
    \varsigma \equiv \den{H}{}{\sigma} &\equiv \bigstar_{(l,f,m) \in \sigma} [ l \mapsto_f m ]\\
\\
\den{}{k}{ \Theta; \Delta ; \Gamma \vdash e : t } &= \forall \theta, \delta, \gamma, \sigma.\ \dom(\Theta) = \dom(\theta) \wedge (\varsigma, \gamma) \in \den{L}{k}{ \Gamma }\theta \wedge \delta \in \den{I}{k}{ \Delta }\theta \Rightarrow \\
                                                 & \qquad \qquad (\varsigma, \gamma(\delta(e))) \in \C{k}{ \theta(t) }
\end{align*}
